Logic/REPEAT/Proofs.lean
@@ -1,0 +1,72 @@
+import Logic.REPEAT.Semantics
+
+namespace Logic.REPEAT
+
+theorem root_in_Q (cft: CFTrace):
+  ε ∈ cft.Q := by
+    exact InQ.root
+
+theorem repeat_entry_in_Q (cft: CFTrace) (s: DynIndex) (i: Nat):
+  DynIndex.line s i ∈ cft.Q →
+  stmt cft (DynIndex.line s i) = some (Stmt.repeat) →
+  InQ cft (DynIndex.line (s $) 0) := by
+    intro hsInQ hrep
+    --intro hrep
+
+    exact InQ.repeat_entry s i hsInQ hrep
+
+theorem valid_tar_implies_valid_cft (cft: CFTrace):
+  wellFormedTar cft → validCFTrace cft := by
+    intro hwellFormedTar
+    simp [wellFormedTar, validCFTrace] at *
+    constructor
+    · exact InQ.root
+    · intro s e args
+      constructor
+      intro hsInQ
+      intro hStmt
+      sorry
+      sorry
+
+
+
+--TODO: IH is too weak
+theorem no_hash_line (cft: CFTrace):
+  ∀ t, InQ cft t →
+  (∀ s i, t ≠ DynIndex.line (s #) i) ∧ -- no line comes after #
+  (∀ s, t ≠ (s #) $) ∧                 -- no dollar comes after #
+  (∀ s, t ≠ (s #) #) := by             -- no hash after hash
+    intro t h
+    --intro h
+    induction h with
+    | root => simp
+    | call s expr args hs hstmt ih =>
+                                      constructor
+                                      · intro s' i heq
+                                        cases heq
+                                        simp[stmt] at *
+
+                                      · constructor
+                                        · intro s heq
+                                          cases heq
+                                        · intro s heq
+                                          cases heq
+    | assign s i v e₀ e₁ hsi hassign ih =>
+                                      simp at *
+                                      exact ih
+    | return_next s i e hsi hreturn ih =>
+                                      simp at *
+                                      exact ih
+    | return_exit s i e hsi hreturn ih =>
+                                      simp at *
+                                      exact ih
+    | repeat_iter s i hsi hrepeat ih =>
+                                      simp at *
+                                      exact ih
+    | repeat_entry s i hsi hrepeat ih =>
+                                      simp at *
+    | repeat_return s hs ih => sorry
+
+    | call_return s i hsi ih => sorry
+
+end Logic.REPEAT
