Logic/REPEAT/Semantics.lean
@@ -1,0 +1,210 @@
+import Mathlib.Data.Set.Basic
+import Logic.REPEAT.Syntax
+
+namespace Logic.REPEAT
+
+
+
+inductive DynIndex where
+  | root : DynIndex
+  | line : DynIndex → Nat → DynIndex
+  | dollar: DynIndex → DynIndex
+  | hash: DynIndex → DynIndex
+deriving DecidableEq
+
+/--
+Encapsulates a control flow trace, which is a triple P = (Q, prompt, tar) where
+* `Q` is a Set of States, represented as `Set DynIndex` => this is defined later inductively
+* `prompt` is the initial call to a procedure
+* `tar` is the call function mapping from states to called procedures
+-/
+structure CFTrace where
+  prompt : Stmt
+  tar : DynIndex → Option Proc
+
+
+/--
+Quasi Execution quadruple Q = (P, seed), where P is a control flow trace and seed provides initial variable values
+-/
+structure QuasiExecution where
+  cft : CFTrace
+  seed : DynIndex → Var → Int → Int
+
+
+/--
+Partial stmt function, which evaluates to the statement at a given dynamic index
+-/
+def stmt (cft: CFTrace) (idx: DynIndex) : Option Stmt :=
+  match idx with
+    | .root => some cft.prompt -- stmt(ε) = prompt, where [] represents ε
+    | .line s i  => -- stmt(s i)
+
+        match cft.tar s with --ctf.tar s is the current procedure
+          | none => none          --shouldn't occur in valid cft (i.e. s i ∈ Q → ∃ p, tar s = some p)
+          | some proc => --TODO: Why no list indices as line numbers?
+              match proc.body.find? (λ ls => ls.line == i) with --extract statement at line i
+                | none => none
+                | some ls => some ls.stmt
+    | _ => none
+
+
+
+--notation for readability
+notation "ε" => DynIndex.root
+notation:max s "$" => DynIndex.dollar s
+notation:max s "#" => DynIndex.hash s
+
+
+/--
+Inductive Proposition defining the states in Q.
+TODO: Currently: On control flow branching at `if e return` both possibilities for val(e) = TRUE and val(e) = FALSE are added.
+-/
+inductive InQ (cft: CFTrace): DynIndex → Prop where
+  -- ε in Q
+  | root: InQ cft ε
+
+  -- if s ∈ Q and stmt (s) is a call `call expr args` then s 0 ∈ Q
+  | call
+    (s: DynIndex)
+    (expr: Expr)
+    (args: List Arg)
+    (hs: InQ cft s) -- s ∈ Q
+    (hstmt: stmt cft s = some (Stmt.call expr args)): --stmt (s) is a call
+
+    InQ cft (DynIndex.line s 0)
+
+  -- if s i ∈ Q and stmt (s i) is an assignment `v[e₀] = e₁`, then s (i+1) ∈ Q
+  | assign
+    (s: DynIndex)
+    (i: Nat)
+    (v: Var)
+    (e₀ e₁: Expr)
+    (hsi: InQ cft (DynIndex.line s i)) -- s i ∈ Q
+    (hassign: stmt cft (DynIndex.line s i) = some (Stmt.assign v e₀ e₁)): -- stmt (s i) is assignment
+
+    InQ cft (DynIndex.line s (i + 1))
+
+  -- if s i ∈ Q and stmt (s i) is a returnIf `if e return` then s (i+1) ∈ Q
+  | return_next
+    (s: DynIndex)
+    (i: Nat)
+    (e: Expr)
+    (hsi: InQ cft (DynIndex.line s i)) -- s i ∈ Q
+    (hreturn: stmt cft (DynIndex.line s i) = some (Stmt.returnIf e)): -- stmt (s i) is return
+
+    InQ cft (DynIndex.line s (i + 1))
+
+  -- if s i ∈ Q and stmt (s i) is a returnIf `if e return` then s # ∈ Q
+  | return_exit
+    (s: DynIndex)
+    (i: Nat)
+    (e: Expr)
+    (hsi: InQ cft (DynIndex.line s i)) -- s i ∈ Q
+    (hreturn: stmt cft (DynIndex.line s i) = some (Stmt.returnIf e)): -- stmt (s i) is return
+
+    InQ cft (s #)
+
+  -- if s i ∈ Q and stmt (s i) is `repeat` then s $ ∈ Q
+  | repeat_iter
+    (s: DynIndex)
+    (i: Nat)
+    (hsi: InQ cft (DynIndex.line s i)) -- s i ∈ Q
+    (hrepeat: stmt cft (DynIndex.line s i) = some (Stmt.repeat)): -- stmt (s i) is repeat
+
+    InQ cft (s $)
+
+  -- if s i ∈ Q and stmt (s i) is `repeat` then s $ 0 ∈ Q
+  | repeat_entry
+    (s: DynIndex)
+    (i: Nat)
+    (hsi: InQ cft (DynIndex.line s i)) -- s i ∈ Q
+    (hrepeat: stmt cft (DynIndex.line s i) = some (Stmt.repeat)): -- stmt (s i) is repeat
+
+    InQ cft (DynIndex.line  (s $) 0)
+
+  -- if s $ # ∈ Q then s # ∈ Q
+  | repeat_return
+    (s: DynIndex)
+    (hs: InQ cft ((s $) #)): -- s $ # ∈ Q
+
+    InQ cft (s #)
+
+  -- if s i # ∈ Q, then s (i+1) ∈ Q
+  | call_return
+    (s: DynIndex)
+    (i: Nat)
+    (hsi: InQ cft  ((DynIndex.line s i) #) ): -- s i # ∈ Q
+
+    InQ cft (DynIndex.line s (i+1))
+
+
+def CFTrace.Q (cft: CFTrace): Set DynIndex :=
+  { s | InQ cft s}
+
+def wellFormedTar (cft: CFTrace): Prop :=
+
+  -- given stmt (s) is a call `call expr args`, tar (s) maps to an arity-matching procedure
+  (∀ s expr args,
+   (s ∈ cft.Q ∧
+    stmt cft s = some (Stmt.call expr args) →
+    ∃ proc, (cft.tar s = some proc ∧ args.length = proc.params.length)
+    ))
+  ∧
+  -- given stmt (s i) is a `repeat`, tar (s $) = tar (s)
+  (∀ s i proc,
+   (DynIndex.line s i ∈ cft.Q ∧
+    stmt cft (DynIndex.line s i) = some (Stmt.repeat) ∧
+    cft.tar s = some proc) →
+    cft.tar (s $) = some proc)
+
+
+
+def validCFTrace (cft: CFTrace) : Prop :=
+    --ε in Q
+    ε ∈ cft.Q
+  ∧
+    -- if s ∈ Q and stmt (s) is a call `call expr args`, then s 0 ∈ Q and tar(s) maps to a arity matching procedure
+    ∀ s expr args,
+    ((s ∈ cft.Q ∧ stmt cft s = some (Stmt.call expr args)) →
+
+      DynIndex.line s 0 ∈ cft.Q ∧
+      ∃ proc, (cft.tar s = some proc ∧ args.length = proc.params.length))
+  ∧
+    -- if s i ∈ Q and stmt(s i) is an assignment `v[e₀] = e₁`, then s (i+1) ∈ Q
+    ∀ s i v e₀ e₁,
+    (DynIndex.line s i ∈ cft.Q ∧
+     stmt cft (DynIndex.line s i) = some (Stmt.assign v e₀ e₁) →
+
+     DynIndex.line s (i + 1) ∈ cft.Q)
+
+  ∧
+    -- if s i ∈ Q and stmt(s i) is a returnIf `if e return ` then either s (i+1) ∈ Q or s # ∈ Q
+    ∀ s i e,
+    (DynIndex.line s i) ∈ cft.Q ∧
+     stmt cft (DynIndex.line s i) = some (Stmt.returnIf e) →
+
+     (DynIndex.line s (i + 1) ∈ cft.Q ∨ s # ∈ cft.Q)
+
+  ∧
+    -- if s i ∈ Q and stmt(s i) is `repeat`, then s $ ∈ Q, s $ 0 ∈ Q and tar(s $) = tar(s)
+    ∀ s i proc,
+    (DynIndex.line s i ∈ cft.Q ∧
+     stmt cft (DynIndex.line s i) = some (Stmt.repeat) ∧
+     cft.tar s = some proc) →
+
+     (s $ ∈ cft.Q ∧
+      DynIndex.line (s $) 0 ∈ cft.Q ∧
+      cft.tar (s $) = some proc)
+  ∧
+    -- if s $ # ∈ Q, then s # ∈ Q
+    ∀ s,
+    (s $) # ∈ cft.Q → s # ∈ cft.Q
+
+  ∧
+    -- if s i # ∈ Q, then s (i + 1) ∈ Q
+    ∀ s i,
+    (DynIndex.line s i) # ∈ cft.Q → DynIndex.line s (i +1) ∈ cft.Q
+
+
+
+end Logic.REPEAT
